Beginnings of small step semantics

proofs/soundness.v
@@ -26,24 +26,140 @@ Definition highOrdSpec : Type := list (string * evtSeq * evtSeq).
 
 Definition contEff : Type := (highOrdSpec * evtSeq).
 
+Inductive value : Set :=
+  | unit
+  | litnum (n:nat)
+  | litbool (b:bool)
+  | var    (s:string)
+  | func   (f:string) (x:string) (e:expr) (* TODO pre/post *)
 
+with handler : Set :=
+  | h_eff (l x:string) (k:value) (e:expr) (h:handler)
+  | h_ret (x:string) (e:expr)
 
-Inductive value : Type := 
-
+with expr : Set :=
+  | val    (v:value)
+  | app    (v1 v2:value)
+  | letIn    (x:string) (e1 e2:expr)
+  | ifElse (v:value) (e1:expr) (e2:expr)
+  | perform (l:string) (v:value)
+  | matchWith (e:expr) (h:handler)
 .
 
+(* v1[v/x] = v2 *)
+(* not mutually recursive because we don't substitute under binders *)
+Definition subst_val (v1 v : value) (x : string) : value :=
+  match v1 with
+  | unit => unit
+  | litnum n => litnum n
+  | litbool b => litbool b
+  | func f y e => func f y e
+  | var y => if string_dec x y then v else v1
+  end.
 
-Inductive expr : Type :=
-| unit
-| litnum (n:nat)
-| var    (s:string)
-| bind   (s:string) (e1:expr) (e2:expr)
-| app    (s:string) (e:expr)
-| binop  (op:string) (e1:expr) (e2:expr)
-| ifElse (v:nat) (e1:expr) (e2:expr)
-| fnDef  (f:string) 
-| closure(f:string) (parm:list string) (e:expr)
+(* h[v/x] = h1 *)
+Fixpoint subst_handler (h:handler) (v : value) (x : string) : handler :=
+  match h with
+  (* TODO deal with variable capture? *)
+  | h_eff l x1 k e h1 =>
+    h_eff l x1 k (subst_expr e v x) (subst_handler h1 v x)
+  | h_ret x e => h_ret x (subst_expr e v x)
+  end
+
+(* e[v/x] = e1 *)
+with subst_expr (e : expr) (v : value) (x : string) : expr :=
+  match e with
+  | val v1 => val (subst_val v1 v x)
+  | app v1 v2 => app (subst_val v1 v x) (subst_val v1 v x)
+  (* TODO deal with variable capture? *)
+  | letIn x e1 e2 => letIn x (subst_expr e1 v x) (subst_expr e2 v x)
+  | ifElse v1 e1 e2 => ifElse (subst_val v1 v x) (subst_expr e1 v x) (subst_expr e2 v x)
+  | perform l v1 => perform l (subst_val v1 v x)
+  | matchWith e1 h => matchWith (subst_expr e1 v x) (subst_handler h v x)
+  end.
+
+Require Export FMapAVL.
+Require Export Coq.Structures.OrderedTypeEx.
+
+Module Map := FMapAVL.Make(String_as_OT).
+
+Notation env := (Map.t value).
+
+Inductive step : expr -> expr -> Prop :=
+| SIfT : forall e1 e2,
+  step (ifElse (litbool true) e1 e2) e1
+| SIfF : forall e1 e2,
+  step (ifElse (litbool false) e1 e2) e1
+| SLet : forall v e e1 x,
+  subst_expr e v x = e1 ->
+  step (letIn x (val v) e) e1
+| SApp : forall f v e e1 x,
+  subst_expr e v x = e1 ->
+  step (app (func f x e) v) e1
+(* TODO match value *)
+(* TODO match perform, after U_l *)
 .
+
+Local Hint Constructors step : core.
+Notation " e1 '-->' e2 " := (step e1 e2) (at level 10).
+
+(* evaluation contexts E *)
+Inductive context : Set :=
+| e_hole
+| e_letIn (x:string) (ctx:context) (e:expr)
+| e_matchWith (ctx:context) (h:handler).
+
+(* TODO U_l evaluation context *)
+
+Inductive sub_context : context -> expr -> expr -> Prop :=
+| ESubHole : forall e,
+  sub_context e_hole e e
+| ESubLet : forall e1 e2 e3 x ctx,
+  sub_context ctx e2 e3 ->
+  sub_context (e_letIn x ctx e1) e2 (letIn x e3 e1)
+| ESubMatch : forall e1 e2 ctx h,
+  sub_context ctx e1 e2 ->
+  sub_context (e_matchWith ctx h) e1 (matchWith e2 h).
+
+Local Hint Constructors sub_context : core.
+
+(* 10 is the maximum it can be to work as an arg of ->...? *)
+Notation " ctx '[' e1 ']' '==' e2 " := (sub_context ctx e1 e2) (at level 10).
+
+Inductive estep : expr -> expr -> Prop :=
+| EStep : forall E c1 c2 C1 C2,
+  (* given a step *)
+  c1 --> c2 ->
+  (* which occurs inside larger exprs C1 and C2 *)
+  E[c1] == C1 ->
+  E[c2] == C2 ->
+  (* C1 can take a step to C2 *)
+  estep C1 C2.
+
+Local Hint Constructors estep : core.
+
+Require Import Coq.Relations.Relation_Operators.
+Local Hint Constructors clos_trans : core.
+Notation estep_star := (clos_trans expr estep).
+
+(* some example programs *)
+
+Definition func_id := func "f" "x" (val (var "x")).
+
+Example ex1 :
+  estep (ifElse (litbool true) (val (litnum 1)) (val (litnum 2))) (val (litnum 1)).
+Proof.
+  eauto.
+Qed.
+
+Example ex2 :
+  estep_star (letIn "x" (letIn "y" (val (litnum 1)) (val (var "y"))) (val (var "x"))) (val (litnum 1)).
+Proof.
+  apply (t_trans _ _ _ (letIn "x" (val (litnum 1)) (val (var "x")))).
+  - eauto 6.
+  - eauto.
+Qed.
+
 (*
 
 differnce: sync - presnet valid for one time cycle 
